<?xml version="1.0" encoding="UTF-8"?>

<!-- 
    WARNING:  THIS IS A WORKING DRAFT ONTOLOGY AND STILL UNDER DEVELOPMENT, this file will change frequently and significantly as development continues
    
    Note:  http://ontology.library.harvard.edu/geo/ is a placeholder (inactive) namespace for the LD4P/L Cartographic Materials "Geospatial and Cartographic Resources Ontology" extension until a proper home is found
	
	last revised: 2017-11-22
  -->

<rdf:RDF
    xmlns="http://ontology.library.harvard.edu/geo/"
    xmlns:bf="http://id.loc.gov/ontologies/bibframe/"
    xmlns:bib="http://bibliotek-o.org/ontology/"
    xmlns:dcterms="http://purl.org/dc/terms/"
    xmlns:owl="http://www.w3.org/2002/07/owl#"
    xmlns:rdf="http://www.w3.org/1999/02/22-rdf-syntax-ns#" 
    xmlns:rdfs="http://www.w3.org/2000/01/rdf-schema#"  
    xmlns:skos="http://www.w3.org/2004/02/skos/core#"
    xmlns:vann="http://purl.org/vocab/vann/"
    xmlns:xsd="http://www.w3.org/2001/XMLSchema#"
    xmlns:foaf="http://xmlns.com/foaf/0.1#"
    >
    
    <!-- ONTOLOGY DECLARATION -->
    
    <owl:Ontology rdf:about="http://ontology.library.harvard.edu/geo/">
        <owl:versionInfo rdf:datatype="http://www.w3.org/2001/XMLSchema#string">Version 0.0</owl:versionInfo>
        <rdfs:label xml:lang="en">Geospatial and Cartographic Resources Ontology: extension ontology for describing cartographic materials</rdfs:label>
        <vann:preferredNamespacePrefix>gcro</vann:preferredNamespacePrefix>
        <rdfs:comment xml:lang="en">Geospatial and Cartographic Resources Ontology is an extension ontology of the bibliotek-o BIBFRAME 2.0 extension ontology produced by the Linked Data for Libraries Cartographic Materials project for use in describing geospatial and cartographic resources</rdfs:comment>
    </owl:Ontology>
    
 
    <!-- CLASSES -->
    
    <!-- Class http://id.loc.gov/ontologies/bibframe/Identifier -->
    
    <owl:Class rdf:about="http://ontology.library.harvard.edu/geo/EpsgCode">
        <rdfs:label xml:lang="en">EPSG Code</rdfs:label>
        <rdfs:subClassOf rdf:resource="http://id.loc.gov/ontologies/bibframe/Identifier"/>
        <skos:definition xml:lang="en">EPSG Dataset Code</skos:definition>
    </owl:Class>
	
	<!-- Class http://id.loc.gov/ontologies/bibframe/Cartography  
    Subclasses of geospatial and cartographic data types -->
	
	<owl:Class rdf:about="http://ontology.library.harvard.edu/geo/Atlases">
	    <rdfs:label xml:lang="en">Atlases</rdfs:label>
        <rdfs:subClassOf rdf:resource="http://id.loc.gov/ontologies/bibframe/Cartography"/>
        <skos:definition xml:lang="en">A collection of maps designed to be kept (bound or loose) in a volume</skos:definition>
    </owl:Class>
	
	<owl:Class rdf:about="http://ontology.library.harvard.edu/geo/CartographicModels">
	    <rdfs:label xml:lang="en">Cartographic Model</rdfs:label>
        <rdfs:subClassOf rdf:resource="http://id.loc.gov/ontologies/bibframe/Cartography"/>
        <skos:definition xml:lang="en">A general category which denotes any three-dimensional representation of an object or geographic area, modeled in any size or medium [not including globes]</skos:definition>
    </owl:Class>
		
	<owl:Class rdf:about="http://ontology.library.harvard.edu/geo/AstronomicalModels">
	    <rdfs:label xml:lang="en">Astronomical Model</rdfs:label>
        <rdfs:subClassOf rdf:resource="http://ontology.library.harvard.edu/geo/CartographicModels"/>
        <skos:definition xml:lang="en">Astronomical models</skos:definition>
    </owl:Class>
	
	<owl:Class rdf:about="http://ontology.library.harvard.edu/geo/ReliefModels">
	    <rdfs:label xml:lang="en">Relief Model</rdfs:label>
        <rdfs:subClassOf rdf:resource="http://ontology.library.harvard.edu/geo/CartographicModels"/>
        <skos:definition xml:lang="en">A map whose surface is shaped to represent the topography in a region. Also called a terrain model</skos:definition>
    </owl:Class>
	
	<owl:Class rdf:about="http://ontology.library.harvard.edu/geo/CartographicProfiles">
	    <rdfs:label xml:lang="en">Cartographic Profile</rdfs:label>
        <rdfs:subClassOf rdf:resource="http://ontology.library.harvard.edu/geo/Cartography"/>
        <skos:definition xml:lang="en">A scale representation of the intersection of a vertical surface (which mayh or may not be a plane) with the surface of the ground, or of the intersection of such a vertical surface with that of a conceptual three-dimensional model representing phenomena having a continuous distribution (e.g. rainfall).  The vertical scale is often exaggerated. (AACR2 mod.)</skos:definition>
    </owl:Class>
	
	<owl:Class rdf:about="http://ontology.library.harvard.edu/geo/CartographicSections">
	    <rdfs:label xml:lang="en">Cartographic Section</rdfs:label>
        <rdfs:subClassOf rdf:resource="http://id.loc.gov/ontologies/bibframe/Cartography"/>
        <skos:definition xml:lang="en">A scale representation of a vertical surface (commonly a plane) displaying both the profile where it intersects the surface of the ground, or some conceptual model, and the underlying structures along the plane of intersection (e.g. a geologic section) (AACR2 mod.)</skos:definition>
    </owl:Class>
		
	<owl:Class rdf:about="http://ontology.library.harvard.edu/geo/GeologicalCrossSections">
	    <rdfs:label xml:lang="en">Geological Cross-section</rdfs:label>
        <rdfs:subClassOf rdf:resource="http://ontology.library.harvard.edu/geo/CartographicSections"/>
        <skos:definition xml:lang="en">A diagram or drawing that shows features transected by a given plane; specif. a vertical section drawn at right angles to the longer axis of a geologic feature, such as as the trend of an orebody, the mean direction of flow of a stream, or the axis of a fossil</skos:definition>
    </owl:Class>
	
	<owl:Class rdf:about="http://ontology.library.harvard.edu/geo/CartographicViews">
	    <rdfs:label xml:lang="en">Cartographic View</rdfs:label>
        <rdfs:subClassOf rdf:resource="http://id.loc.gov/ontologies/bibframe/Cartography"/>
        <skos:definition xml:lang="en">A perspective representation of cities or landscapes</skos:definition>
    </owl:Class>
	
	<owl:Class rdf:about="http://ontology.library.harvard.edu/geo/AerialViews">
	    <rdfs:label xml:lang="en">Aerial View</rdfs:label>
        <rdfs:subClassOf rdf:resource="http://ontology.library.harvard.edu/geo/CartographicViews"/>
        <skos:definition xml:lang="en">Representations of cities or landscapes portrayed as if viewed from above</skos:definition>
    </owl:Class>
	
	<owl:Class rdf:about="http://ontology.library.harvard.edu/geo/Panorama">
	    <rdfs:label xml:lang="en">Panorama</rdfs:label>
        <rdfs:subClassOf rdf:resource="http://ontology.library.harvard.edu/geo/CartographicViews"/>
        <skos:definition xml:lang="en">A perspective representation of the landscape in which the detail is shown as if projected onto a vertical plane or onto the insides of a cylinder centered vertically on the observer. (Ency. Dict. of Cart.)</skos:definition>
    </owl:Class>
	
	<owl:Class rdf:about="http://ontology.library.harvard.edu/geo/WormsEyeViews">
	    <rdfs:label xml:lang="en">Worm's Eye View</rdfs:label>
        <rdfs:subClassOf rdf:resource="http://ontology.library.harvard.edu/geo/CartographicViews"/>
        <skos:definition xml:lang="en">Representations of cities or landscapes portrayed as if viewed from a very low viewpoint.</skos:definition>
    </owl:Class>
	
	<owl:Class rdf:about="http://ontology.library.harvard.edu/geo/DigitalCartographicResources">
	    <rdfs:label xml:lang="en">Digital Cartographic Resources</rdfs:label>
        <rdfs:subClassOf rdf:resource="http://id.loc.gov/ontologies/bibframe/Cartography"/>
        <skos:definition xml:lang="en">Digital cartographic resource</skos:definition>
    </owl:Class>
	
	<owl:Class rdf:about="http://ontology.library.harvard.edu/geo/ScannedCartographicResources">
	    <rdfs:label xml:lang="en">Scanned Cartographic Resource</rdfs:label>
        <rdfs:subClassOf rdf:resource="http://ontology.library.harvard.edu/geo/DigitalCartographicResources"/>
        <skos:definition xml:lang="en">An analog resources that has been scanned for digital viewing as a static/non-interactive image</skos:definition>
    </owl:Class>
	
	<owl:Class rdf:about="http://ontology.library.harvard.edu/geo/StaticDigitalCartographicResources">
	    <rdfs:label xml:lang="en">Static Digital Cartographic Resource</rdfs:label>
        <rdfs:subClassOf rdf:resource="http://ontology.library.harvard.edu/geo/DigitalCartographicResources"/>
        <skos:definition xml:lang="en">Born-digital cartographic resource that is static</skos:definition>
    </owl:Class>
	
	<owl:Class rdf:about="http://ontology.library.harvard.edu/geo/InteractiveDigitalCartographicResources">
	    <rdfs:label xml:lang="en">Interactive Digital Cartographic Resource</rdfs:label>
        <rdfs:subClassOf rdf:resource="http://ontology.library.harvard.edu/geo/DigitalCartographicResources"/>
        <skos:definition xml:lang="en">Born-digital cartographic resource that is interactive</skos:definition>
    </owl:Class>
	
	<owl:Class rdf:about="http://ontology.library.harvard.edu/geo/Ephemerides">
	    <rdfs:label xml:lang="en">Ephemerides</rdfs:label>
        <rdfs:subClassOf rdf:resource="http://id.loc.gov/ontologies/bibframe/Cartography"/>
        <skos:definition xml:lang="en">Ephemeris plural ephemerides: a tabular statement of the assigned places of a celestial body for regular intervals. Table of the positions of celestial bodies at regular intervals, often with supplementary information. Constructed as early as the 4th century BC, ephemerides are still essential to astronomers and navigators. Modern ephemerides are calculated, with heavy computing and careful checking, after a mathematical description of a heavenly body's observed motion has been evolved. Various national ephemerides are published regularly; the U.S. ephemeris, first published in 1852, became the best and is now published jointly with the U.K. as The Astronomical Almanac.</skos:definition>
    </owl:Class>
	
	<owl:Class rdf:about="http://ontology.library.harvard.edu/geo/Gazetteers">
	    <rdfs:label xml:lang="en">Gazetteer</rdfs:label>
        <rdfs:subClassOf rdf:resource="http://id.loc.gov/ontologies/bibframe/Cartography"/>
        <skos:definition xml:lang="en">A gazetteer is a geographical dictionary or directory, an important reference for information about places and place names, used in conjunction with a map or a full atlas. It typically contains information concerning the geographical makeup of a country, region, or continent as well as the social statistics and physical features, such as mountains, waterways, or roads.</skos:definition>
    </owl:Class>
	
	<owl:Class rdf:about="http://ontology.library.harvard.edu/geo/GeospatialDigitalData">
	    <rdfs:label xml:lang="en">Geospatial Digital Data</rdfs:label>
        <rdfs:subClassOf rdf:resource="http://id.loc.gov/ontologies/bibframe/Cartography"/>
        <skos:definition xml:lang="en">Digital geospatial data</skos:definition>
    </owl:Class>
	
	<owl:Class rdf:about="http://ontology.library.harvard.edu/geo/VectorData">
	    <rdfs:label xml:lang="en">Vector Data</rdfs:label>
        <rdfs:subClassOf rdf:resource="http://ontology.library.harvard.edu/geo/GeospatialDigitalData"/>
        <skos:definition xml:lang="en">A data structure used to represent linear geographic features. Features are made of ordered lists of x, y or x, y, z coordinates and are represented by points, lines, or polygons; points connect to become lines, and lines connect to become polygons. Attributes are associated with each feature.</skos:definition>
    </owl:Class>
	
	<owl:Class rdf:about="http://ontology.library.harvard.edu/geo/RasterData">
	    <rdfs:label xml:lang="en">Raster Data</rdfs:label>
        <rdfs:subClassOf rdf:resource="http://ontology.library.harvard.edu/geo/GeospatialDigitalData"/>
        <skos:definition xml:lang="en">Data that are based on a cellular grid structure composed of rows and columns (a raster). Each grid cell or pixel is referenced by an x, y coordinate and is stored as an identifier to which additional attributes may be attached. Groups of cells with the same value represent map features.</skos:definition>
	</owl:Class>
	
	<owl:Class rdf:about="http://ontology.library.harvard.edu/geo/GeoreferencedCartographicResources">
	    <rdfs:label xml:lang="en">Georeferenced Cartographic Resource</rdfs:label>
        <rdfs:subClassOf rdf:resource="http://ontology.library.harvard.edu/geo/GeospatialDigitalData"/>
        <skos:definition xml:lang="en">A scanned, paper map or cartographic resource that has been fit to real world coordinates using a GIS and is enabled for spatial display in a digital environment</skos:definition>
	</owl:Class>
	
	<owl:Class rdf:about="http://ontology.library.harvard.edu/geo/GeospatialDatabases">
	    <rdfs:label xml:lang="en">Geospatial Database</rdfs:label>
        <rdfs:subClassOf rdf:resource="http://ontology.library.harvard.edu/geo/GeospatialDigitalData"/>
        <skos:definition xml:lang="en">A database with geospatial data</skos:definition>
	</owl:Class>
	
	<owl:Class rdf:about="http://ontology.library.harvard.edu/geo/Globes">
	    <rdfs:label xml:lang="en">Globe</rdfs:label>
        <rdfs:subClassOf rdf:resource="http://id.loc.gov/ontologies/bibframe/Cartography"/>
        <skos:definition xml:lang="en">A spherical representation of the earth, a celestial body, or the heavens</skos:definition>
    </owl:Class>
	
	<owl:Class rdf:about="http://ontology.library.harvard.edu/geo/CelestialGlobes">
	    <rdfs:label xml:lang="en">Celestial Globe</rdfs:label>
        <rdfs:subClassOf rdf:resource="http://ontology.library.harvard.edu/geo/Globes"/>
        <skos:definition xml:lang="en">A spherical representation of a celestial body, or the heavens</skos:definition>
    </owl:Class>
	
	<owl:Class rdf:about="http://ontology.library.harvard.edu/geo/TerrestrialGlobes">
	    <rdfs:label xml:lang="en">Terrestrial Globe</rdfs:label>
        <rdfs:subClassOf rdf:resource="http://ontology.library.harvard.edu/geo/Globes"/>
        <skos:definition xml:lang="en">A spherical representation of the earth</skos:definition>
    </owl:Class>
	
	<owl:Class rdf:about="http://ontology.library.harvard.edu/geo/Maps">
	    <rdfs:label xml:lang="en">Map</rdfs:label>
        <rdfs:subClassOf rdf:resource="http://id.loc.gov/ontologies/bibframe/Cartography"/>
        <skos:definition xml:lang="en">A graphic representation, usually on a plane surface and at an established scale, of natural and manmade features on or under the surface of the earth or other planetary body. 
            The features are positioned as accurately as possible, usually relative to a coordinate reference system. Also, a graphic representation of a part or the whole of the celestial sphere) physical map</skos:definition>
    </owl:Class>
	
	<!-- Subclasses of Maps -->
	
	<owl:Class rdf:about="http://ontology.library.harvard.edu/geo/AeronauticalCharts">
	    <rdfs:label xml:lang="en">Aeronautical Charts</rdfs:label>
        <rdfs:subClassOf rdf:resource="http://ontology.library.harvard.edu/geo/Maps"/>
		<skos:altLabel xml:lang="en">Navigational Charts</skos:altLabel>
        <skos:definition xml:lang="en">Maps giving information intended for use in air navigation, such as compass rose, isogonic lines, location of landing fields, beacons, hazards to air navigation, etc.</skos:definition>
    </owl:Class>
	
	<owl:Class rdf:about="http://ontology.library.harvard.edu/geo/BottleCharts">
	    <rdfs:label xml:lang="en">Bottle-Charts</rdfs:label>
        <rdfs:subClassOf rdf:resource="http://ontology.library.harvard.edu/geo/Maps"/>
        <skos:definition xml:lang="en">A chart of ocean surface currents to show the track of sealed bottles thrown from ships into the sea</skos:definition>
    </owl:Class>
	
 	<owl:Class rdf:about="http://ontology.library.harvard.edu/geo/CadastralMaps">
	    <rdfs:label xml:lang="en">Cadastral Maps</rdfs:label>
        <rdfs:subClassOf rdf:resource="http://ontology.library.harvard.edu/geo/Maps"/>
		<skos:altLabel xml:lang="en">Plan Diagrams</skos:altLabel>
		<skos:altLabel xml:lang="en">Plan Maps</skos:altLabel>
		<skos:altLabel xml:lang="en">Plat Books</skos:altLabel>
		<skos:altLabel xml:lang="en">Plat Diagrams</skos:altLabel>
		<skos:altLabel xml:lang="en">Plot Diagrams</skos:altLabel>
		<skos:altLabel xml:lang="en">Plot Maps</skos:altLabel>
		<skos:altLabel xml:lang="en">Property Maps</skos:altLabel>
		<skos:altLabel xml:lang="en">Protraction Maps</skos:altLabel>
        <skos:definition xml:lang="en">A map showing the boundaries of subdivisions of land, usually with the bearings and lengths thereof and the areas of individual tracts, for purposes of describing and recording ownership. A cadastral map may also show culture, drainage, and other features affecting the value and use of the land; also known as property map</skos:definition>
    </owl:Class>
	
 	<owl:Class rdf:about="http://ontology.library.harvard.edu/geo/CelestialCharts">
	    <rdfs:label xml:lang="en">Celestial Charts</rdfs:label>
        <rdfs:subClassOf rdf:resource="http://ontology.library.harvard.edu/geo/Maps"/>
        <skos:definition xml:lang="en">A map of representation of the celestial sphere, or of some part thereof</skos:definition>
    </owl:Class>
	
	<owl:Class rdf:about="http://ontology.library.harvard.edu/geo/ComparativeMaps">
	    <rdfs:label xml:lang="en">Comparative Maps</rdfs:label>
        <rdfs:subClassOf rdf:resource="http://ontology.library.harvard.edu/geo/Maps"/>
		<skos:altLabel xml:lang="en">Comparative Area Maps</skos:altLabel>
        <skos:definition xml:lang="en">A map comparing the relative size of two or more geographic areas</skos:definition>
    </owl:Class>
	
 	<owl:Class rdf:about="http://ontology.library.harvard.edu/geo/EarlyMaps">
	    <rdfs:label xml:lang="en">Early Maps</rdfs:label>
        <rdfs:subClassOf rdf:resource="http://ontology.library.harvard.edu/geo/Maps"/>
        <skos:definition xml:lang="en">Generally refers to maps created before 1801</skos:definition>
    </owl:Class>
	
 	<owl:Class rdf:about="http://ontology.library.harvard.edu/geo/EthnographicMaps">
	    <rdfs:label xml:lang="en">Ethnographic Maps</rdfs:label>
        <rdfs:subClassOf rdf:resource="http://ontology.library.harvard.edu/geo/Maps"/>
		<skos:altLabel xml:lang="en">Anthropological Maps</skos:altLabel>
		<skos:altLabel xml:lang="en">Ethnographical Maps</skos:altLabel>
		<skos:altLabel xml:lang="en">Ethnological Maps</skos:altLabel>
        <skos:definition xml:lang="en">Maps relating to ethnology, anthropology, and the diversity of humanity and human culture in general</skos:definition>
    </owl:Class>
	
 	<owl:Class rdf:about="http://ontology.library.harvard.edu/geo/FireInsuranceMaps">
	    <rdfs:label xml:lang="en">Fire Insurance Maps</rdfs:label>
        <rdfs:subClassOf rdf:resource="http://ontology.library.harvard.edu/geo/Maps"/>
		<skos:altLabel xml:lang="en">Fire Insurance Risk Maps</skos:altLabel>
		<skos:altLabel xml:lang="en">Risk Maps, Fire Insurance</skos:altLabel>
		<skos:altLabel xml:lang="en">Sanborn Fire Insurance Maps</skos:altLabel>
		<skos:altLabel xml:lang="en">Sanborn Maps</skos:altLabel>
        <skos:definition xml:lang="en">Maps intended for use in calculating fire insurance risks prepared primarily for the use of fire insurance underwriters, which show detailed, accurate, and up-to-date information on potential fire hazards and risks for individual residences and commercial and industrial installations in urban and suburban areas.  Information shown includes the type of interior and exterior construction material, dimensions, and heights of buildings, block, lot and building numbers, occupancy of buildings, and such fire protection facilities as watermains, fire hydrants, and fire alarm boxes</skos:definition>
    </owl:Class>
	
 	<owl:Class rdf:about="http://ontology.library.harvard.edu/geo/FlowMaps">
	    <rdfs:label xml:lang="en">Flow Maps</rdfs:label>
        <rdfs:subClassOf rdf:resource="http://ontology.library.harvard.edu/geo/Maps"/>
		<skos:altLabel xml:lang="en">Cartograms, Linear</skos:altLabel>
		<skos:altLabel xml:lang="en">Dynamic Maps</skos:altLabel>
		<skos:altLabel xml:lang="en">Flow Line Maps</skos:altLabel>
		<skos:altLabel xml:lang="en">Line Maps, Flow</skos:altLabel>
		<skos:altLabel xml:lang="en">Linear Cartograms</skos:altLabel>
        <skos:definition xml:lang="en">Flow maps in cartography are by definition of Phan (2005) "a mix of maps and flow charts, that show the movement of objects from one location to another, such as the number of people in a migration, the amount of goods being traded, or the number of packets in a network." Flow maps according to Harris (1999) "can be used to show movement of almost anything, including tangible things such as people, products, natural resources, weather, etc, as well as intangible things such as know-how, talent, credit of goodwill"</skos:definition>
    </owl:Class>
	
 	<owl:Class rdf:about="http://ontology.library.harvard.edu/geo/GeologicalMaps">
	    <rdfs:label xml:lang="en">Geological Maps</rdfs:label>
        <rdfs:subClassOf rdf:resource="http://ontology.library.harvard.edu/geo/Maps"/>
		<skos:altLabel xml:lang="en">Geologic Maps</skos:altLabel>
		<skos:altLabel xml:lang="en">Geology Maps</skos:altLabel>
        <skos:definition xml:lang="en">A map showing the structure and composition of the earth's crust</skos:definition>
    </owl:Class>
	
 	<owl:Class rdf:about="http://ontology.library.harvard.edu/geo/GoresMaps">
	    <rdfs:label xml:lang="en">Gores (Maps)</rdfs:label>
        <rdfs:subClassOf rdf:resource="http://ontology.library.harvard.edu/geo/Maps"/>
		<skos:altLabel xml:lang="en">Globe Gores</skos:altLabel>
        <skos:definition xml:lang="en">Triangular or lune-shaped segment that can be fitted to the surface of a sphere with little distortion or deformation</skos:definition>
    </owl:Class>
	
 	<owl:Class rdf:about="http://ontology.library.harvard.edu/geo/GravityAnomalyMaps">
	    <rdfs:label xml:lang="en">Gravity Anomaly Maps</rdfs:label>
        <rdfs:subClassOf rdf:resource="http://ontology.library.harvard.edu/geo/Maps"/>
		<skos:altLabel xml:lang="en">Gravity maps</skos:altLabel>
        <skos:definition xml:lang="en">Gravity anomaly maps depict the difference between theoretical computed gravity values and observed gravity values for a region of the earth's crust</skos:definition>
    </owl:Class>
	
 	<owl:Class rdf:about="http://ontology.library.harvard.edu/geo/IndexMaps">
	    <rdfs:label xml:lang="en">Index Maps</rdfs:label>
        <rdfs:subClassOf rdf:resource="http://ontology.library.harvard.edu/geo/Maps"/>
		<skos:altLabel xml:lang="en">Key Maps</skos:altLabel>
        <skos:definition xml:lang="en">A map showing where to find collections of related data such as other maps, aerial photographs, statistical data, or descriptions of terrain.  Also called a key map</skos:definition>
    </owl:Class>
	
 	<owl:Class rdf:about="http://ontology.library.harvard.edu/geo/ManuscriptMaps">
	    <rdfs:label xml:lang="en">Manuscript Maps</rdfs:label>
        <rdfs:subClassOf rdf:resource="http://ontology.library.harvard.edu/geo/Maps"/>
        <skos:definition xml:lang="en">The original drawing of a map as compiled or constructed from various data such as ground surveys and photographs</skos:definition>
    </owl:Class>
	
 	<owl:Class rdf:about="http://ontology.library.harvard.edu/geo/MappaeMundi">
	    <rdfs:label xml:lang="en">Mappae Mundi</rdfs:label>
        <rdfs:subClassOf rdf:resource="http://ontology.library.harvard.edu/geo/Maps"/>
		<skos:altLabel xml:lang="en">Mappa Mundi</skos:altLabel>
		<skos:altLabel xml:lang="en">Mappamundi</skos:altLabel>
        <skos:definition xml:lang="en">Used for medieval (usually circular) world maps, made between the fall of the western Roman empire in the later years of the 5th century AD and the end of the 15th century</skos:definition>
    </owl:Class>
	
 	<owl:Class rdf:about="http://ontology.library.harvard.edu/geo/MentalMaps">
	    <rdfs:label xml:lang="en">Mental Maps</rdfs:label>
        <rdfs:subClassOf rdf:resource="http://ontology.library.harvard.edu/geo/Maps"/>
        <skos:definition xml:lang="en">A mental map can best be explained as a visual display, inside a person's head, showing where a person has traveled. A mental map shows what the person knows about the location and the uniqueness of a place. No mental map is alike. Every human has his or her own mental map</skos:definition>
    </owl:Class>
	
 	<owl:Class rdf:about="http://ontology.library.harvard.edu/geo/MeteorologicalCharts">
	    <rdfs:label xml:lang="en">Meteorological Charts</rdfs:label>
        <rdfs:subClassOf rdf:resource="http://ontology.library.harvard.edu/geo/Maps"/>
        <skos:definition xml:lang="en">A chart giving information about the weather</skos:definition>
    </owl:Class>
	
 	<owl:Class rdf:about="http://ontology.library.harvard.edu/geo/MilitaryMaps">
	    <rdfs:label xml:lang="en"Military Maps></rdfs:label>
        <rdfs:subClassOf rdf:resource="http://ontology.library.harvard.edu/geo/Maps"/>
        <skos:definition xml:lang="en">A map designed particularly for military use</skos:definition>
    </owl:Class>

	<owl:Class rdf:about="http://ontology.library.harvard.edu/geo/MineMaps">
	    <rdfs:label xml:lang="en">Mine Maps</rdfs:label>
        <rdfs:subClassOf rdf:resource="http://ontology.library.harvard.edu/geo/Maps"/>
        <skos:definition xml:lang="en">Maps recording mining activity, either specific mines or broader areas of mining. Maps can be topographic or cross-sectional in nature</skos:definition>
    </owl:Class>
	
 	<owl:Class rdf:about="http://ontology.library.harvard.edu/geo/MiniatureMaps">
	    <rdfs:label xml:lang="en">Miniature Maps</rdfs:label>
        <rdfs:subClassOf rdf:resource="http://ontology.library.harvard.edu/geo/Maps"/>
        <skos:definition xml:lang="en">Generally, any map with an size of 150 square centimeters or less</skos:definition>
    </owl:Class>
	
 	<owl:Class rdf:about="http://ontology.library.harvard.edu/geo/NauticalCharts">
	    <rdfs:label xml:lang="en">Nautical Charts</rdfs:label>
        <rdfs:subClassOf rdf:resource="http://ontology.library.harvard.edu/geo/Maps"/>
		<skos:altLabel xml:lang="en">Hydrographic Charts</skos:altLabel>
		<skos:altLabel xml:lang="en">Navigation Charts</skos:altLabel>
		<skos:altLabel xml:lang="en">Navigation Maps</skos:altLabel>
		<skos:altLabel xml:lang="en">Pilot Charts</skos:altLabel>
        <skos:definition xml:lang="en">A chart designed for use in navigating ships, boats, or other watercraft</skos:definition>
    </owl:Class>
	
 	<owl:Class rdf:about="http://ontology.library.harvard.edu/geo/OutlineMaps">
	    <rdfs:label xml:lang="en">Outline Maps</rdfs:label>
        <rdfs:subClassOf rdf:resource="http://ontology.library.harvard.edu/geo/Maps"/>
		<skos:altLabel xml:lang="en">Base maps</skos:altLabel>
        <skos:definition xml:lang="en">A map showing just enough geographic information to permit the correct placement of additional details.  Outline maps correspond to what were at one time known as base maps; they usually show only cast lines, principal rivers, major civil boundaries, and large cities.  As much space as possible is left for placing the particular details or data desired.  An outline map presents less detail than what is now known as a base map</skos:definition>
    </owl:Class>
	
 	<owl:Class rdf:about="http://ontology.library.harvard.edu/geo/Photomaps">
	    <rdfs:label xml:lang="en">Photomaps</rdfs:label>
        <rdfs:subClassOf rdf:resource="http://ontology.library.harvard.edu/geo/Maps"/>
		<skos:altLabel xml:lang="en">Orthophoto Maps</skos:altLabel>
		<skos:altLabel xml:lang="en">Orthophotomaps</skos:altLabel>
		<skos:altLabel xml:lang="en">Photo Maps</skos:altLabel>
		<skos:altLabel xml:lang="en">Photographic Maps</skos:altLabel>
        <skos:definition xml:lang="en">A map made from assembling photographs and adding appropriate information such as a reference system, grid, labels, scale, and so forth</skos:definition>
    </owl:Class>
	
 	<owl:Class rdf:about="http://ontology.library.harvard.edu/geo/PhysicalMaps">
	    <rdfs:label xml:lang="en">Physical Maps</rdfs:label>
        <rdfs:subClassOf rdf:resource="http://ontology.library.harvard.edu/geo/Maps"/>
        <skos:definition xml:lang="en">A map representing the surface of the land or the floor of the oceans. In addition to representing the relief, physical maps show some natural phenomena such as oceanic currents, swamps, sands and deserts. Man-made structures or vegetation are not shown</skos:definition>
    </owl:Class>
	
 	<owl:Class rdf:about="http://ontology.library.harvard.edu/geo/PictorialMaps">
	    <rdfs:label xml:lang="en">Pictorial Maps</rdfs:label>
        <rdfs:subClassOf rdf:resource="http://ontology.library.harvard.edu/geo/Maps"/>
        <skos:definition xml:lang="en">Maps that depict a given territory with a more artistic rather than technical style, usually showing an area as if viewed from above at an oblique angle</skos:definition>
    </owl:Class>
	
 	<owl:Class rdf:about="http://ontology.library.harvard.edu/geo/PortolanCharts">
        <rdfs:subClassOf rdf:resource="http://ontology.library.harvard.edu/geo/Maps"/>
        <skos:definition xml:lang="en">A class of early coastal charts capable of navigational use which feature a network of interconnected lines (usually termed rhumb lines); place names written inland at right angles to the coast; drawn in ink on one or more skins following established color conventions; with coastlines shown in a general fashion with bays and headlines exaggerated and navigational hazards marked with crosses and dots</skos:definition>
    </owl:Class>
	
 	<owl:Class rdf:about="http://ontology.library.harvard.edu/geo/QuadrangleMaps">
	    <rdfs:label xml:lang="en">Quadrangle Maps</rdfs:label>
        <rdfs:subClassOf rdf:resource="http://ontology.library.harvard.edu/geo/Maps"/>
		<skos:altLabel xml:lang="en">Quad Maps</skos:altLabel>
		<skos:altLabel xml:lang="en">Quadrangular Maps</skos:altLabel>
        <skos:definition xml:lang="en">Maps that cover a rectangular or nearly rectangular region defined by four specified points</skos:definition>
    </owl:Class>
	
 	<owl:Class rdf:about="http://ontology.library.harvard.edu/geo/RemoteSensingMaps">
	    <rdfs:label xml:lang="en">Remote-sensing Maps</rdfs:label>
        <rdfs:subClassOf rdf:resource="http://ontology.library.harvard.edu/geo/Maps"/>
        <skos:definition xml:lang="en">High-resolution topographic, bathymetric, or habitat maps created using remote-sensing applications which generate images by means of reflected or emitted electromagnetic energy</skos:definition>
    </owl:Class>
	
 	<owl:Class rdf:about="http://ontology.library.harvard.edu/geo/RoadMaps">
	    <rdfs:label xml:lang="en">Road Maps</rdfs:label>
        <rdfs:subClassOf rdf:resource="http://ontology.library.harvard.edu/geo/Maps"/>
		<skos:altLabel xml:lang="en">Roadmaps</skos:altLabel>
		<skos:altLabel xml:lang="en">Street maps</skos:altLabel>
        <skos:definition xml:lang="en">A map, usually at medium or small scale, showing the roads in a region</skos:definition>
    </owl:Class>
	
 	<owl:Class rdf:about="http://ontology.library.harvard.edu/geo/StatisticalMaps">
	    <rdfs:label xml:lang="en">Statistical Maps</rdfs:label>
        <rdfs:subClassOf rdf:resource="http://ontology.library.harvard.edu/geo/Maps"/>
		<skos:altLabel xml:lang="en">Maps of residuals</skos:altLabel>
		<skos:altLabel xml:lang="en">Residuals, Maps of</skos:altLabel>
        <skos:definition xml:lang="en">A special type of map in which the variation in quantity of a factor such as rainfall, population, or crops in a geographic area is indicated; a dot map is one type</skos:definition>
    </owl:Class>
	
 	<owl:Class rdf:about="http://ontology.library.harvard.edu/geo/StickCharts">
	    <rdfs:label xml:lang="en">Stick Charts</rdfs:label>
        <rdfs:subClassOf rdf:resource="http://ontology.library.harvard.edu/geo/Maps"/>
        <skos:definition xml:lang="en">Charts made by Pacific Islanders that indicate the pattern of swells and wave masses caused by wind</skos:definition>
    </owl:Class>
	
 	<owl:Class rdf:about="http://ontology.library.harvard.edu/geo/StripMaps">
	    <rdfs:label xml:lang="en">Strip Maps</rdfs:label>
        <rdfs:subClassOf rdf:resource="http://ontology.library.harvard.edu/geo/Maps"/>
        <skos:definition xml:lang="en">A map (as for an aviator) showing only a narrow band of territory (as 500 miles long and ten miles wide</skos:definition>
    </owl:Class>
	
 	<owl:Class rdf:about="http://ontology.library.harvard.edu/geo/ThematicMaps">
	    <rdfs:label xml:lang="en">Thematic Maps</rdfs:label>
        <rdfs:subClassOf rdf:resource="http://ontology.library.harvard.edu/geo/Maps"/>
		<skos:altLabel xml:lang="en">Chloropleth Maps</skos:altLabel>
		<skos:altLabel xml:lang="en">Single-topic Maps</skos:altLabel>
		<skos:altLabel xml:lang="en">Special-purpose Maps</skos:altLabel>
		<skos:altLabel xml:lang="en">Topical Maps</skos:altLabel>
        <skos:definition xml:lang="en">A map whose principal purpose is depicting information other than that about the Earth's physical surface. Also called a topical map. Among the kinds of information shown on thematic maps are density of population, kind or amount of crops grown, types of soil, amount of rainfall and administrative subdivisions</skos:definition>
    </owl:Class>
	
 	<owl:Class rdf:about="http://ontology.library.harvard.edu/geo/TopographicMaps">
	    <rdfs:label xml:lang="en">Topographic Maps</rdfs:label>
        <rdfs:subClassOf rdf:resource="http://ontology.library.harvard.edu/geo/Maps"/>
		<skos:altLabel xml:lang="en">Hypsographic Maps</skos:altLabel>
		<skos:altLabel xml:lang="en">Hypsometric Maps</skos:altLabel>
		<skos:altLabel xml:lang="en">Relief Maps</skos:altLabel>
		<skos:altLabel xml:lang="en">Topo Maps</skos:altLabel>
		<skos:altLabel xml:lang="en">Topographical Maps</skos:altLabel>
        <skos:definition xml:lang="en">A map showing the horizontal and vertical locations of the natural and man-made features represented. Also called a relief map. Uses numbered contour lines or comparable symbols to show mountains, valleys and plains; a map whose principle purpose is to portray and identify the natural and artificial features on the Earth's surface as faithfully as possible within the limitations imposed by scale</skos:definition>
    </owl:Class>
	
 	<owl:Class rdf:about="http://ontology.library.harvard.edu/geo/TouristMaps">
	    <rdfs:label xml:lang="en">Tourist Maps</rdfs:label>
        <rdfs:subClassOf rdf:resource="http://ontology.library.harvard.edu/geo/Maps"/>
        <skos:definition xml:lang="en">Maps designed for tourists</skos:definition>
    </owl:Class>
	
 	<owl:Class rdf:about="http://ontology.library.harvard.edu/geo/UpsideDownMaps">
	    <rdfs:label xml:lang="en">Upside-down Maps</rdfs:label>
        <rdfs:subClassOf rdf:resource="http://ontology.library.harvard.edu/geo/Maps"/>
		<skos:altLabel xml:lang="en">Reversed Maps</skos:altLabel>
		<skos:altLabel xml:lang="en">South-up Maps</skos:altLabel>
		<skos:altLabel xml:lang="en">Upsidedown Maps</skos:altLabel>
        <skos:definition xml:lang="en">Maps in which the orientation has been reversed and south appears at the top</skos:definition>
    </owl:Class>
	
 	<owl:Class rdf:about="http://ontology.library.harvard.edu/geo/WallMaps">
	    <rdfs:label xml:lang="en">Wall Maps</rdfs:label>
        <rdfs:subClassOf rdf:resource="http://ontology.library.harvard.edu/geo/Maps"/>
        <skos:definition xml:lang="en">A map designed to be mounted or displayed on a wall, generally has devices on map to assist in hanging</skos:definition>
    </owl:Class>
	
 	<owl:Class rdf:about="http://ontology.library.harvard.edu/geo/WorldMaps">
	    <rdfs:label xml:lang="en">World Maps</rdfs:label>
        <rdfs:subClassOf rdf:resource="http://ontology.library.harvard.edu/geo/Maps"/>
        <skos:definition xml:lang="en">A world map is a map of most or all of the surface of the Earth. World maps form a distinctive category of maps due to the problem of projection. Maps by necessity distort the presentation of the earth's surface. These distortions reach extremes in a world map. The many ways of projecting the earth reflect diverse technical and aesthetic goals for world maps</skos:definition>
    </owl:Class>
	
 	<owl:Class rdf:about="http://ontology.library.harvard.edu/geo/ZoningMaps">
	    <rdfs:label xml:lang="en">Zoning Maps</rdfs:label>
        <rdfs:subClassOf rdf:resource="http://ontology.library.harvard.edu/geo/Maps"/>
		<skos:altLabel xml:lang="en">Zoning District Maps</skos:altLabel>
        <skos:definition xml:lang="en">Zoning maps show the boundaries of zoning districts throughout the city</skos:definition>
    </owl:Class>
	
	<!-- / end of / Subclasses of Maps -->
	
	<owl:Class rdf:about="http://ontology.library.harvard.edu/geo/RemoteSensingImages">
	    <rdfs:label xml:lang="en">Remote Sensing Image</rdfs:label>
        <rdfs:subClassOf rdf:resource="http://id.loc.gov/ontologies/bibframe/Cartography"/>
        <skos:definition xml:lang="en">Images of planetary surfaces created by means of reflected or emitted electromagnetic energy</skos:definition>
    </owl:Class>
	
	<owl:Class rdf:about="http://ontology.library.harvard.edu/geo/AerialPhotographs">
	    <rdfs:label xml:lang="en">Aerial Photograph</rdfs:label>
        <rdfs:subClassOf rdf:resource="http://ontology.library.harvard.edu/geo/RemoteSensingImages"/>
        <skos:definition xml:lang="en">Images of planetary surfaces created by means of reflected or emitted electromagnetic energy</skos:definition>
    </owl:Class>
	
		<!-- Class http://id.loc.gov/ontologies/bibframe/Scale 
    Adding subclasses of cartographic scales -->
	
	<owl:Class rdf:about="http://ontology.library.harvard.edu/geo/HorizontalScale">
	    <rdfs:label xml:lang="en">Horizontal Scale</rdfs:label>
        <rdfs:subClassOf rdf:resource="http://id.loc.gov/ontologies/bibframe/Scale"/>
        <skos:definition xml:lang="en">Horizontal scale</skos:definition>
    </owl:Class>
	
	<owl:Class rdf:about="http://ontology.library.harvard.edu/geo/VerticalScale">
	    <rdfs:label xml:lang="en">Vertical Scale</rdfs:label>
        <rdfs:subClassOf rdf:resource="http://id.loc.gov/ontologies/bibframe/Scale"/>
        <skos:definition xml:lang="en">Vertical scale</skos:definition>
    </owl:Class>
	
	<owl:Class rdf:about="http://ontology.library.harvard.edu/geo/NotToScale">
	    <rdfs:label xml:lang="en">Not to Scale</rdfs:label>
        <rdfs:subClassOf rdf:resource="http://id.loc.gov/ontologies/bibframe/Scale"/>
        <skos:definition xml:lang="en">Not to scale</skos:definition>
    </owl:Class>
	
	<owl:Class rdf:about="http://ontology.library.harvard.edu/geo/ScaleIndeterminable">
	    <rdfs:label xml:lang="en">Scale Indeterminable</rdfs:label>
        <rdfs:subClassOf rdf:resource="http://id.loc.gov/ontologies/bibframe/Scale"/>
        <skos:definition xml:lang="en">Scale indeterminable</skos:definition>
    </owl:Class>
	
	<owl:Class rdf:about="http://ontology.library.harvard.edu/geo/ScaleNotDetermined">
	    <rdfs:label xml:lang="en">Scale Not Determined</rdfs:label>
        <rdfs:subClassOf rdf:resource="http://id.loc.gov/ontologies/bibframe/Scale"/>
        <skos:definition xml:lang="en">Scale not determined</skos:definition>
    </owl:Class>
	
	<owl:Class rdf:about="http://ontology.library.harvard.edu/geo/ScalesDiffer">
	    <rdfs:label xml:lang="en">Scales Differ</rdfs:label>
        <rdfs:subClassOf rdf:resource="http://id.loc.gov/ontologies/bibframe/Scale"/>
        <skos:definition xml:lang="en">Scales differ</skos:definition>
    </owl:Class>
	
	<owl:Class rdf:about="http://ontology.library.harvard.edu/geo/ScaleVaries">
	    <rdfs:label xml:lang="en">Scale Varies</rdfs:label>
        <rdfs:subClassOf rdf:resource="http://id.loc.gov/ontologies/bibframe/Scale"/>
        <skos:definition xml:lang="en">Scale varies</skos:definition>
    </owl:Class>
	
	<!-- Class http://id.loc.gov/ontologies/bibframe/Scale 
    Adding classes related to cartographic scales -->
	
	<owl:Class rdf:about="http://ontology.library.harvard.edu/geo/ScaleAccuracy">
	    <rdfs:label xml:lang="en">Scale Accuracy</rdfs:label>
        <skos:definition xml:lang="en">Scale accuracy</skos:definition>
    </owl:Class>
	
	<owl:Class rdf:about="http://ontology.library.harvard.edu/geo/ScaleSource">
	    <rdfs:label xml:lang="en">Scale Source</rdfs:label>
        <skos:definition xml:lang="en">Source of the map scale</skos:definition>
    </owl:Class>
	
	<!-- Class http://ontology.library.harvard.edu/geo/Relief 
    Adding Relief class and its subclasses (subclasses based primarily on MARC Map format relief codes (008/18-21) / (006/01-04) -->
	
	<owl:Class rdf:about="http://ontology.library.harvard.edu/geo/Relief">
        <rdfs:label xml:lang="en">Relief</rdfs:label>
        <skos:definition xml:lang="en">Inequalities of elevation and the configuration of land features on the surface of the Earth that may be represented on maps or charts by contours, hypsometric tints, shading, spot elevations, or hachures. Also encompasses the depiction or indication of underwater topography, or the depths and shapes of underwater terrain</skos:definition>
    </owl:Class>
	
	<owl:Class rdf:about="http://ontology.library.harvard.edu/geo/LandRelief">
        <rdfs:label xml:lang="en">Land Relief</rdfs:label>
        <rdfs:subClassOf rdf:resource="http://ontology.library.harvard.edu/geo/Relief"/>
        <skos:definition xml:lang="en">Inequalities of elevation and the configuration of land features on the surface of the Earth that may be represented on maps or charts by contours, hypsometric tints, shading, spot elevations, or hachures</skos:definition>
    </owl:Class>
	
	<owl:Class rdf:about="http://ontology.library.harvard.edu/geo/Contours">
        <rdfs:label xml:lang="en">Contours</rdfs:label>
        <rdfs:subClassOf rdf:resource="http://ontology.library.harvard.edu/geo/LandRelief"/>
        <skos:definition xml:lang="en">Relief shown by contours</skos:definition>
		<rdfs:comment xml:lang="en">MARC Map format relief code: a</rdfs:comment>
    </owl:Class>
	
	<owl:Class rdf:about="http://ontology.library.harvard.edu/geo/Shading">
        <rdfs:label xml:lang="en">Shading</rdfs:label>
        <rdfs:subClassOf rdf:resource="http://ontology.library.harvard.edu/geo/LandRelief"/>
        <skos:definition xml:lang="en">Relief shown by shading (generally of a single color)</skos:definition>
		<rdfs:comment xml:lang="en">MARC Map format relief code: b</rdfs:comment>
    </owl:Class>
	
	<owl:Class rdf:about="http://ontology.library.harvard.edu/geo/GradientTints">
        <rdfs:label xml:lang="en">Gradient Tints</rdfs:label>
        <rdfs:subClassOf rdf:resource="http://ontology.library.harvard.edu/geo/LandRelief"/>
        <skos:definition xml:lang="en">Relief shown by gradient tints</skos:definition>
		<rdfs:comment xml:lang="en">MARC Map format relief code: c</rdfs:comment>
    </owl:Class>
	
	<owl:Class rdf:about="http://ontology.library.harvard.edu/geo/Hachures">
        <rdfs:label xml:lang="en">Hachures</rdfs:label>
        <rdfs:subClassOf rdf:resource="http://ontology.library.harvard.edu/geo/LandRelief"/>
        <skos:definition xml:lang="en">Relief shown by hachures (short lines which follow the direction of maximum slope)</skos:definition>
		<rdfs:comment xml:lang="en">MARC Map format relief code: d</rdfs:comment>
    </owl:Class>
	
	<owl:Class rdf:about="http://ontology.library.harvard.edu/geo/FormLines">
        <rdfs:label xml:lang="en">Form Lines</rdfs:label>
        <rdfs:subClassOf rdf:resource="http://ontology.library.harvard.edu/geo/LandRelief"/>
        <skos:definition xml:lang="en">Land relief shown by form lines</skos:definition>
		<rdfs:comment xml:lang="en">MARC Map format relief code: f</rdfs:comment>
    </owl:Class>
	
	<owl:Class rdf:about="http://ontology.library.harvard.edu/geo/SpotHeights">
        <rdfs:label xml:lang="en">Spot Heights</rdfs:label>
        <rdfs:subClassOf rdf:resource="http://ontology.library.harvard.edu/geo/LandRelief"/>
        <skos:definition xml:lang="en">Relief shown by spot heights</skos:definition>
		<rdfs:comment xml:lang="en">MARC Map format relief code: g</rdfs:comment>
    </owl:Class>
	
	<owl:Class rdf:about="http://ontology.library.harvard.edu/geo/Pictorially">
        <rdfs:label xml:lang="en">Pictorially</rdfs:label>
        <rdfs:subClassOf rdf:resource="http://ontology.library.harvard.edu/geo/LandRelief"/>
        <skos:definition xml:lang="en">Land forms and other topographic features shown in the correct planimetric position by pictorial symbols representing their appearance from a high oblique view</skos:definition>
		<rdfs:comment xml:lang="en">MARC Map format relief code: i</rdfs:comment>
    </owl:Class>
	
	<owl:Class rdf:about="http://ontology.library.harvard.edu/geo/LandForms">
        <rdfs:label xml:lang="en">Land Forms</rdfs:label>
        <rdfs:subClassOf rdf:resource="http://ontology.library.harvard.edu/geo/LandRelief"/>
        <skos:definition xml:lang="en">Relief shown by land forms</skos:definition>
		<rdfs:comment xml:lang="en">MARC Map format relief code: j</rdfs:comment>
    </owl:Class>
	
	<owl:Class rdf:about="http://ontology.library.harvard.edu/geo/RockDrawings">
        <rdfs:label xml:lang="en">Rock Drawings</rdfs:label>
        <rdfs:subClassOf rdf:resource="http://ontology.library.harvard.edu/geo/LandRelief"/>
        <skos:definition xml:lang="en">Relief rock drawing</skos:definition>
		<rdfs:comment xml:lang="en">MARC Map format relief code: m</rdfs:comment>
    </owl:Class>
	
	<owl:Class rdf:about="http://ontology.library.harvard.edu/geo/WaterRelief">
        <rdfs:label xml:lang="en">Water Relief</rdfs:label>
        <rdfs:subClassOf rdf:resource="http://ontology.library.harvard.edu/geo/Relief"/>
        <skos:definition xml:lang="en">The depiction or indication of underwater topography, or the depths and shapes of underwater terrain</skos:definition>
		<rdfs:comment xml:lang="en">MARC Map format relief code: </rdfs:comment>
    </owl:Class>
	
	<owl:Class rdf:about="http://ontology.library.harvard.edu/geo/BathymetricTints">
        <rdfs:label xml:lang="en">Bathymetric Tints</rdfs:label>
        <rdfs:subClassOf rdf:resource="http://ontology.library.harvard.edu/geo/WaterRelief"/>
        <skos:definition xml:lang="en">Underwater relief shown by bathymetric tints</skos:definition>
		<rdfs:comment xml:lang="en">MARC Map format relief code: c</rdfs:comment>
    </owl:Class>
	
	<owl:Class rdf:about="http://ontology.library.harvard.edu/geo/BathymetricIsolines">
        <rdfs:label xml:lang="en">Bathymetric Isolines</rdfs:label>
        <rdfs:subClassOf rdf:resource="http://ontology.library.harvard.edu/geo/WaterRelief"/>
        <skos:definition xml:lang="en">Underwater relief (depth) shown by isolines (lines that represent constant depths)</skos:definition>
		<rdfs:comment xml:lang="en">MARC Map format relief code: k</rdfs:comment>
    </owl:Class>
	
	<owl:Class rdf:about="http://ontology.library.harvard.edu/geo/BathymetricSoundings">
        <rdfs:label xml:lang="en">Bathymetric Soundings</rdfs:label>
        <rdfs:subClassOf rdf:resource="http://ontology.library.harvard.edu/geo/WaterRelief"/>
		<skos:altLabel xml:lang="en">Bathymetry/Soundings</skos:altLabel>
        <skos:definition xml:lang="en">Underwater relief (depth) shown by soundings</skos:definition>
		<rdfs:comment xml:lang="en">MARC Map format relief code: e</rdfs:comment>
    </owl:Class>
	
	<owl:Class rdf:about="http://ontology.library.harvard.edu/geo/BathymetricFormLines">
        <rdfs:label xml:lang="en">Bathymetric Form Lines</rdfs:label>
        <rdfs:subClassOf rdf:resource="http://ontology.library.harvard.edu/geo/WaterRelief"/>
        <skos:definition xml:lang="en">Underwater relief shown by form lines</skos:definition>
		<rdfs:comment xml:lang="en">MARC Map format relief code: f</rdfs:comment>
    </owl:Class>
	
	<owl:Class rdf:about="http://ontology.library.harvard.edu/geo/NoRelief">
        <rdfs:label xml:lang="en">No Relief</rdfs:label>
        <rdfs:subClassOf rdf:resource="http://ontology.library.harvard.edu/geo/Relief"/>
        <skos:definition xml:lang="en">No relief shown</skos:definition>
		<rdfs:comment xml:lang="en">MARC Map format relief code: #</rdfs:comment>
    </owl:Class>
	
	<owl:Class rdf:about="http://ontology.library.harvard.edu/geo/NoLandRelief">
        <rdfs:label xml:lang="en">No Land Relief</rdfs:label>
        <rdfs:subClassOf rdf:resource="http://ontology.library.harvard.edu/geo/NoRelief"/>
        <skos:definition xml:lang="en">No land relief shown</skos:definition>
    </owl:Class>
	
	<owl:Class rdf:about="http://ontology.library.harvard.edu/geo/NoWaterRelief">
        <rdfs:label xml:lang="en">No Water Relief</rdfs:label>
        <rdfs:subClassOf rdf:resource="http://ontology.library.harvard.edu/geo/NoRelief"/>
        <skos:definition xml:lang="en">No underwater relief shown</skos:definition>
    </owl:Class>
	
	<owl:Class rdf:about="http://ontology.library.harvard.edu/geo/OtherRelief">
        <rdfs:label xml:lang="en">Other Relief</rdfs:label>
        <rdfs:subClassOf rdf:resource="http://ontology.library.harvard.edu/geo/Relief"/>
        <skos:definition xml:lang="en">None of the other defined codes are appropriate</skos:definition>
		<rdfs:comment xml:lang="en">MARC Map format relief code: z</rdfs:comment>
    </owl:Class>
	
	<owl:Class rdf:about="http://ontology.library.harvard.edu/geo/NoAttemptToCode">
        <rdfs:label xml:lang="en">No Attempt To Code</rdfs:label>
        <rdfs:subClassOf rdf:resource="http://ontology.library.harvard.edu/geo/Relief"/>
        <skos:definition xml:lang="en">Relief not determined</skos:definition>
		<rdfs:comment xml:lang="en">MARC Map format relief code: ||||</rdfs:comment>
    </owl:Class>
	
	<owl:Class rdf:about="http://ontology.library.harvard.edu/geo/ReliefNotDetermined">
        <rdfs:label xml:lang="en">Relief Not Determined</rdfs:label>
        <rdfs:subClassOf rdf:resource="http://ontology.library.harvard.edu/geo/Relief"/>
        <skos:definition xml:lang="en">Relief not determined</skos:definition>
    </owl:Class>
		
    <!-- OBJECT PROPERTIES -->
    
    <owl:ObjectProperty rdf:about="http://ontology.library.harvard.edu/geo/isGeometryOf">
        <rdfs:label xml:lang="en">Is Geometry of</rdfs:label>
        <owl:inverseOf rdf:resource="http://www.opengis.net/ont/geosparql#hasGeometry"/>
    </owl:ObjectProperty>
    
    <owl:ObjectProperty rdf:about="http://ontology.library.harvard.edu/geo/isProjectionOf">
        <rdfs:label xml:lang="en">Is Projection of</rdfs:label>
        <owl:inverseOf rdf:resource="http://id.loc.gov/ontologies/bibframe/projection"/>
    </owl:ObjectProperty>    
	
	<owl:ObjectProperty rdf:about="http://ontology.library.harvard.edu/geo/scaleAccuracy">
	    <rdfs:label xml:lang="en">Has scale accuracy</rdfs:label>
        <skos:definition xml:lang="en">Accuracy of the scale statement</skos:definition>
        <rdfs:domain rdf:resource="http://id.loc.gov/ontologies/bibframe/Scale"/> 
		<rdfs:range rdf:resource="http://ontology.library.harvard.edu/geo/ScaleAccuracy"/>
    </owl:ObjectProperty>
	
	<owl:ObjectProperty rdf:about="http://ontology.library.harvard.edu/geo/scaleSource">
	    <rdfs:label xml:lang="en">Scale source</rdfs:label>
        <skos:definition xml:lang="en">Has scale source</skos:definition>
        <rdfs:domain rdf:resource="http://id.loc.gov/ontologies/bibframe/Scale"/> 
		<rdfs:range rdf:resource="http://ontology.library.harvard.edu/geo/ScaleSource"/>
    </owl:ObjectProperty>
	
	<owl:ObjectProperty rdf:about="http://ontology.library.harvard.edu/geo/relief">
        <rdfs:label xml:lang="en">Has relief</rdfs:label>
        <skos:definition xml:lang="en">Depicts or indicates relief</skos:definition>
		<rdfs:domain rdf:resource="http://id.loc.gov/ontologies/bibframe/Cartography"/>
		<rdfs:range rdf:resource="http://ontology.library.harvard.edu/geo/Relief"/>
    </owl:ObjectProperty>	
	
	<!-- DATA PROPERTIES -->
    
	<owl:DatatypeProperty rdf:about="http://ontology.library.harvard.edu/geo/representativeFractionDenominator">
	    <rdfs:label xml:lang="en">Representative Fraction Denominator</rdfs:label>
	    <skos:definition xml:lang="en">The denominator of the scale's representative fraction</skos:definition>
	    <rdfs:domain rdf:resource="http://id.loc.gov/ontologies/bibframe/Scale"/>
        <rdfs:range rdf:resource="http://www.w3.org/2000/01/rdf-schema#Literal"/>
	</owl:DatatypeProperty>
        
    <!-- NAMED INDIVIDUALS -->
    
    <!-- Type http://id.loc.gov/ontologies/bibframe/Projection 
    Adding Individuals MARC coded projection types: https://www.loc.gov/marc/bibliographic/bd008p.html -->
    
    <owl:NamedIndividual rdf:about="http://ontology.library.harvard.edu/geo/Mercator">
        <rdf:type rdf:resource="http://id.loc.gov/ontologies/bibframe/Projection"/>
        <rdfs:label xml:lang="en">Mercator</rdfs:label>
        <skos:definition xml:lang="en">A projection of a map of the world onto a cylinder in such a way that all the parallels of latitude have the same length as the equator, used especially for marine charts and certain climatological maps.</skos:definition>
        <dcterms:issued></dcterms:issued>
        <dcterms:modified></dcterms:modified>
    </owl:NamedIndividual>

    <owl:NamedIndividual rdf:about="http://ontology.library.harvard.edu/geo/ProjectionEpsg4326">
        <rdf:type rdf:resource="http://id.loc.gov/ontologies/bibframe/Projection"/>
        <rdfs:label xml:lang="en">WGS 84</rdfs:label>
        <skos:definition xml:lang="en">World Geodetic System 1984.</skos:definition>
        <bf:identifiedBy rdf:resource="http://ontology.library.harvard.edu/geo/EpsgCode4326"/>
        <dcterms:issued></dcterms:issued>
        <dcterms:modified></dcterms:modified>
    </owl:NamedIndividual>

    <!-- Type http://ontology.library.harvard.edu/geo/EpsgCode
    Individuals of type  EpsgCode -->
    
    <owl:NamedIndividual rdf:about="http://ontology.library.harvard.edu/geo/EpsgCode4326">
        <rdf:type rdf:resource="http://ontology.library.harvard.edu/geo/EpsgCode"/>
        <rdfs:label xml:lang="en">WGS 84</rdfs:label>
        <skos:definition xml:lang="en">World Geodetic System 1984</skos:definition>
        <bf:identifies rdf:resource="http://ontology.library.harvard.edu/geo/ProjectionEpsg4326"/>
        <foaf:page>http://epsg.io/4326</foaf:page>
        <rdf:value>4326</rdf:value>
        <dcterms:issued></dcterms:issued>
        <dcterms:modified></dcterms:modified>
    </owl:NamedIndividual>
	
    <!-- Type http://ontology.library.harvard.edu/geo/ScaleAccuracy
    Individuals of type  ScaleAccuracy -->
    
    <owl:NamedIndividual rdf:about="http://ontology.library.harvard.edu/geo/ExplicitScale">
        <rdf:type rdf:resource="http://ontology.library.harvard.edu/geo/ScaleAccuracy"/>
        <rdfs:label xml:lang="en">Explicit scale</rdfs:label>
        <skos:definition xml:lang="en">Scale as stated on the cartographic resource</skos:definition>
        <dcterms:issued></dcterms:issued>
        <dcterms:modified></dcterms:modified>
    </owl:NamedIndividual>
	
	<owl:NamedIndividual rdf:about="http://ontology.library.harvard.edu/geo/ApproximateScale">
        <rdf:type rdf:resource="http://ontology.library.harvard.edu/geo/ScaleAccuracy"/>
	    <rdfs:label xml:lang="en">Approximate scale</rdfs:label>
	    <skos:definition xml:lang="en">Approximate scale of cartographic resource</skos:definition>
        <dcterms:issued></dcterms:issued>
        <dcterms:modified></dcterms:modified>
    </owl:NamedIndividual>
	
	<owl:NamedIndividual rdf:about="http://ontology.library.harvard.edu/geo/InaccurateScale">
        <rdf:type rdf:resource="http://ontology.library.harvard.edu/geo/ScaleAccuracy"/>
	    <rdfs:label xml:lang="en">Inaccurate scale</rdfs:label>
	    <skos:definition xml:lang="en">Inaccurate scale of cartographic resource</skos:definition>
        <dcterms:issued></dcterms:issued>
        <dcterms:modified></dcterms:modified>
    </owl:NamedIndividual>
	
	<owl:NamedIndividual rdf:about="http://ontology.library.harvard.edu/geo/ScaleAccuracyUnknown">
        <rdf:type rdf:resource="http://ontology.library.harvard.edu/geo/ScaleAccuracy"/>
	    <rdfs:label xml:lang="en">Scale accuracy unknown</rdfs:label>
	    <skos:definition xml:lang="en">Scale accuracy unknown</skos:definition>
        <dcterms:issued></dcterms:issued>
        <dcterms:modified></dcterms:modified>
    </owl:NamedIndividual>
	
	<!-- Type http://ontology.library.harvard.edu/geo/ScaleSource
    Individuals of type  ScaleSource -->
    
    <owl:NamedIndividual rdf:about="http://ontology.library.harvard.edu/geo/RepresentativeFraction">
        <rdf:type rdf:resource="http://ontology.library.harvard.edu/geo/ScaleSource"/>
        <rdfs:label xml:lang="en">Representative Fraction</rdfs:label>
        <skos:definition xml:lang="en">Source of scale is the representative fraction</skos:definition>
        <dcterms:issued></dcterms:issued>
        <dcterms:modified></dcterms:modified>
    </owl:NamedIndividual>
	
	<owl:NamedIndividual rdf:about="http://ontology.library.harvard.edu/geo/VerbalStatement">
        <rdf:type rdf:resource="http://ontology.library.harvard.edu/geo/ScaleSource"/>
	    <rdfs:label xml:lang="en">Verbal Statement</rdfs:label>
	    <skos:definition xml:lang="en">Source of scale is a verbal statement</skos:definition>
        <dcterms:issued></dcterms:issued>
        <dcterms:modified></dcterms:modified>
    </owl:NamedIndividual>
	
	<owl:NamedIndividual rdf:about="http://ontology.library.harvard.edu/geo/ScaleBar">
        <rdf:type rdf:resource="http://ontology.library.harvard.edu/geo/ScaleSource"/>
	    <rdfs:label xml:lang="en">Scale Bar</rdfs:label>
	    <skos:definition xml:lang="en">Source of scale is the scale bar</skos:definition>
        <dcterms:issued></dcterms:issued>
        <dcterms:modified></dcterms:modified>
    </owl:NamedIndividual>
	
	<owl:NamedIndividual rdf:about="http://ontology.library.harvard.edu/geo/CalculatedFromPrimarySource">
        <rdf:type rdf:resource="http://ontology.library.harvard.edu/geo/ScaleSource"/>
	    <rdfs:label xml:lang="en">Scale calculated</rdfs:label>
	    <skos:definition xml:lang="en">Source of scale is calculated from the primary source</skos:definition>
        <dcterms:issued></dcterms:issued>
        <dcterms:modified></dcterms:modified>
    </owl:NamedIndividual>
	
	<owl:NamedIndividual rdf:about="http://ontology.library.harvard.edu/geo/DerivedOther">
        <rdf:type rdf:resource="http://ontology.library.harvard.edu/geo/ScaleSource"/>
	    <rdfs:label xml:lang="en">Scale derived</rdfs:label>
	    <skos:definition xml:lang="en">Source of scale is derived from an external resource</skos:definition>
        <dcterms:issued></dcterms:issued>
        <dcterms:modified></dcterms:modified>
    </owl:NamedIndividual>
    
    
    <!-- Type http://bib.ld4l.org/ontology/hasSource 
    Adding individuals of MARC coded cartographic data sources: https://www.loc.gov/standards/sourcelist/cartographic-data.html  -->
    
    <owl:NamedIndividual rdf:about="http://ontology.library.harvard.edu/geo/Bound">
        <rdf:type rdf:resource="http://id.loc.gov/ontologies/bibframe/Source"/>
        <rdfs:label xml:lang="en">Bounding Box (Klokan Technologies)</rdfs:label>
        <skos:definition xml:lang="en">The Klokan Technologies Bounding Box Tool.</skos:definition>
        <dcterms:issued></dcterms:issued>
        <dcterms:modified></dcterms:modified>
    </owl:NamedIndividual>
	
</rdf:RDF>
